viper-total-heaps/TotalConsistencyProperties.thy
@@ -2,7 +2,7 @@ theory TotalConsistencyProperties
   imports TotalSemanticsCore TotalSemantics
 begin
 
-\<comment> \<open>Local variable assignment preserves state consistency.\<close>
+\<comment> \<open>Local variable assignment preserves internal state consistency.\<close>
 
 lemma var_assignment_preserves_state_consistency:
   assumes "get_total_full \<omega> = \<phi>"
@@ -16,7 +16,7 @@ proof -
   thus ?thesis using assms(2) by auto
 qed
 
-\<comment> \<open>Unfold statement preserves state consistency.\<close>
+\<comment> \<open>Unfold statement preserves internal state consistency.\<close>
 
 lemma unfold_preserves_state_consistency:
   assumes "get_total_full \<omega> = \<phi>"
@@ -45,7 +45,7 @@ proof -
   qed
 qed
 
-\<comment> \<open>Field assignment preserves state consistency.\<close>
+\<comment> \<open>Field assignment preserves internal state consistency.\<close>
 
 lemma field_assignment_preserves_state_consistency:
   assumes "get_total_full \<omega> = \<phi>"
@@ -62,5 +62,15 @@ proof -
   thus ?thesis using assms(2)
     by (simp add: total_heap_consistent_def)
 qed
+
+\<comment> \<open>A fraction of a consistent total state is external consistent.\<close>
+
+lemma fraction_consistent_external:
+    fixes frac :: preal
+  assumes "consistent_external ctxt \<omega> (pred_id,vs) p"
+      and "0 < frac \<and> frac < 1"
+      and "nm = nested_mask_multiply (get_nm_total_full \<omega>) frac"
+    shows "consistent_external ctxt (update_nm_total_full \<omega> nm) (pred_id,vs) (p * frac)"
+  oops
 
 end
